Superposition_Calculus/Clause_Typing.thy
@@ -1,0 +1,42 @@
+theory Clause_Typing
+  imports Typing Uprod_Extra Multiset_Extra Clausal_Calculus_Extra
+begin
+
+locale mulitset_typing_lifting = typing_lifting where to_set = set_mset
+begin
+
+lemma is_welltyped_add_mset: 
+  "is_welltyped (add_mset sub M) \<longleftrightarrow> is_welltyped_sub sub \<and> is_welltyped M"
+  by (simp add: is_welltyped_def)
+
+lemma is_welltyped_plus: 
+  "is_welltyped (C + D) \<longleftrightarrow> is_welltyped C \<and> is_welltyped D"
+  by (auto simp: is_welltyped_def)
+
+end
+
+locale clause_typing =
+  "term": explicit_typing term_typed term_welltyped
+  for term_typed term_welltyped
+begin
+
+sublocale atom: uniform_explicit_typing_lifting where 
+  typed_sub = term_typed and 
+  welltyped_sub = term_welltyped and
+  to_set = set_uprod
+  by unfold_locales (rule set_uprod_not_empty)
+
+sublocale literal: uniform_explicit_typing_lifting where 
+  typed_sub = atom.typed and 
+  welltyped_sub = atom.welltyped and
+  to_set = "\<lambda>l. {atm_of l}"
+  by unfold_locales simp
+
+sublocale clause: mulitset_typing_lifting where 
+  is_typed_sub = literal.is_typed and 
+  is_welltyped_sub = literal.is_welltyped
+  by unfold_locales
+
+end
+
+end
