Superposition_Calculus/Ground_Superposition_Welltypedness_Preservation.thy
@@ -1,114 +1,143 @@
 theory Ground_Superposition_Welltypedness_Preservation
-  imports Ground_Superposition Ground_Type_System
+  imports Ground_Superposition Ground_Typing
 begin
 
-lemma (in ground_superposition_calculus) ground_superposition_preserves_typing:
+locale ground_superposition_welltypedness_preservation = 
+  ground_superposition_calculus where select = select + 
+  ground_typing where \<F> = \<F>
+for 
+  select :: "'f gatom clause \<Rightarrow> 'f gatom clause" and
+  \<F> :: "('f, 'ty) fun_types"
+begin
+
+lemma ground_superposition_preserves_typing:
   assumes
     step: "ground_superposition D E C" and
-    wt_D: "welltyped\<^sub>c \<F> D" and
-    wt_E: "welltyped\<^sub>c \<F> E"
-  shows "welltyped\<^sub>c \<F> C"
+    wt_D: "clause.is_welltyped D" and
+    wt_E: "clause.is_welltyped E"
+  shows "clause.is_welltyped C"
   using step
 proof (cases D E C rule: ground_superposition.cases)
   case hyps: (ground_superpositionI L\<^sub>E E' L\<^sub>D D' \<P> \<kappa> t u t')
   show ?thesis
     unfolding \<open>C = add_mset (\<P> (Upair \<kappa>\<langle>t'\<rangle>\<^sub>G u)) (E' + D')\<close>
-    unfolding welltyped\<^sub>c_add_mset welltyped\<^sub>c_plus
+    unfolding clause.is_welltyped_add_mset clause.is_welltyped_plus
   proof (intro conjI)
-    have "\<exists>\<tau>. welltyped \<F> \<kappa>\<langle>t\<rangle>\<^sub>G \<tau> \<and> welltyped \<F> u \<tau>"
+    have "\<exists>\<tau>. term.welltyped \<kappa>\<langle>t\<rangle>\<^sub>G \<tau> \<and> term.welltyped u \<tau>"
     proof -
-      have "welltyped\<^sub>l \<F> L\<^sub>E"
+      have "literal.is_welltyped L\<^sub>E"
         using wt_E
-        unfolding \<open>E = add_mset L\<^sub>E E'\<close> welltyped\<^sub>c_add_mset
+        unfolding \<open>E = add_mset L\<^sub>E E'\<close> clause.is_welltyped_add_mset
         by argo
-      hence "welltyped\<^sub>a \<F> (Upair \<kappa>\<langle>t\<rangle>\<^sub>G u)"
+
+      hence "atom.is_welltyped (Upair \<kappa>\<langle>t\<rangle>\<^sub>G u)"
         using \<open>\<P> \<in> {Pos, Neg}\<close>
-        unfolding \<open>L\<^sub>E = \<P> (Upair \<kappa>\<langle>t\<rangle>\<^sub>G u)\<close> welltyped\<^sub>l_def
+        unfolding \<open>L\<^sub>E = \<P> (Upair \<kappa>\<langle>t\<rangle>\<^sub>G u)\<close> literal.typing_defs atom.typing_defs
         by auto
+
       thus ?thesis
-        unfolding welltyped\<^sub>a_def by simp
+        unfolding atom.typing_defs 
+        by simp
     qed
 
-    moreover have "\<exists>\<tau>. welltyped \<F> t \<tau> \<and> welltyped \<F> t' \<tau>"
+    moreover have "\<exists>\<tau>. term.welltyped t \<tau> \<and> term.welltyped t' \<tau>"
     proof -
-      have "welltyped\<^sub>l \<F> L\<^sub>D"
+      have "literal.is_welltyped L\<^sub>D"
         using wt_D
-        unfolding \<open>D = add_mset L\<^sub>D D'\<close> welltyped\<^sub>c_add_mset
+        unfolding \<open>D = add_mset L\<^sub>D D'\<close> clause.is_welltyped_add_mset
         by argo
-      hence "welltyped\<^sub>a \<F> (Upair t t')"
+
+      hence "atom.is_welltyped (Upair t t')"
         using \<open>\<P> \<in> {Pos, Neg}\<close>
-        unfolding \<open>L\<^sub>D = t \<approx> t'\<close> welltyped\<^sub>l_def
+        unfolding \<open>L\<^sub>D = t \<approx> t'\<close> literal.typing_defs atom.typing_defs
         by auto
+
       thus ?thesis
-        unfolding welltyped\<^sub>a_def by simp
+        unfolding atom.typing_defs
+        by simp
     qed
 
-    ultimately have "\<exists>\<tau>. welltyped \<F> \<kappa>\<langle>t'\<rangle>\<^sub>G \<tau> \<and> welltyped \<F> u \<tau>"
-      using gctxt_apply_term_preserves_typing[of \<F> \<kappa> t _ _ t']
+    ultimately have "\<exists>\<tau>. term.welltyped \<kappa>\<langle>t'\<rangle>\<^sub>G \<tau> \<and> term.welltyped u \<tau>"
+      using term.welltyped_context_compatible
       by blast
-    hence "welltyped\<^sub>a \<F> (Upair \<kappa>\<langle>t'\<rangle>\<^sub>G u)"
-      unfolding welltyped\<^sub>a_def by simp
-    thus "welltyped\<^sub>l \<F> (\<P> (Upair \<kappa>\<langle>t'\<rangle>\<^sub>G u))"
-      unfolding welltyped\<^sub>l_def
+
+    hence "atom.is_welltyped (Upair \<kappa>\<langle>t'\<rangle>\<^sub>G u)"
+      unfolding atom.typing_defs
+      by simp
+
+    thus "literal.is_welltyped (\<P> (Upair \<kappa>\<langle>t'\<rangle>\<^sub>G u))"
+      unfolding literal.typing_defs atom.typing_defs
       using \<open>\<P> \<in> {Pos, Neg}\<close> by auto
   next
-    show "welltyped\<^sub>c \<F> E'"
+    show "clause.is_welltyped E'"
       using wt_E
-      unfolding \<open>E = add_mset L\<^sub>E E'\<close> welltyped\<^sub>c_add_mset
+      unfolding \<open>E = add_mset L\<^sub>E E'\<close> clause.is_welltyped_add_mset
       by argo
   next
-    show "welltyped\<^sub>c \<F> D'"
+    show "clause.is_welltyped D'"
       using wt_D
-      unfolding \<open>D = add_mset L\<^sub>D D'\<close> welltyped\<^sub>c_add_mset
+      unfolding \<open>D = add_mset L\<^sub>D D'\<close> clause.is_welltyped_add_mset
       by argo
   qed
 qed
 
-lemma (in ground_superposition_calculus) ground_eq_resolution_preserves_typing:
+lemma ground_eq_resolution_preserves_typing:
   assumes
     step: "ground_eq_resolution D C" and
-    wt_D: "welltyped\<^sub>c \<F> D"
-  shows "welltyped\<^sub>c \<F> C"
+    wt_D: "clause.is_welltyped D"
+  shows "clause.is_welltyped C"
   using step
 proof (cases D C rule: ground_eq_resolution.cases)
   case (ground_eq_resolutionI L D' t)
   thus ?thesis
     using wt_D
-    unfolding welltyped\<^sub>c_def
+    unfolding clause.typing_defs
     by simp
 qed
 
-lemma (in ground_superposition_calculus) ground_eq_factoring_preserves_typing:
+lemma ground_eq_factoring_preserves_typing:
   assumes
     step: "ground_eq_factoring D C" and
-    wt_D: "welltyped\<^sub>c \<F> D"
-  shows "welltyped\<^sub>c \<F> C"
+    wt_D: "clause.is_welltyped D"
+  shows "clause.is_welltyped C"
   using step
 proof (cases D C rule: ground_eq_factoring.cases)
   case (ground_eq_factoringI L\<^sub>1 L\<^sub>2 D' t t' t'')
-  hence "welltyped\<^sub>l \<F> (t \<approx> t')" and "welltyped\<^sub>l \<F> (t \<approx> t'')" and "welltyped\<^sub>c \<F> D'"
+
+  hence 
+    "literal.is_welltyped (t \<approx> t')" and 
+    "literal.is_welltyped (t \<approx> t'')" and 
+    "clause.is_welltyped D'"
     unfolding atomize_conj
-    using wt_D welltyped\<^sub>c_add_mset by metis
+    using wt_D clause.is_welltyped_add_mset 
+    by metis
 
-  hence "\<exists>\<tau>. welltyped \<F> t \<tau> \<and> welltyped \<F> t' \<tau>" "\<exists>\<tau>. welltyped \<F> t \<tau> \<and> welltyped \<F> t'' \<tau>"
-    unfolding atomize_conj welltyped\<^sub>l_def welltyped\<^sub>a_def by simp
+  hence 
+    "\<exists>\<tau>. term.welltyped t \<tau> \<and> term.welltyped t' \<tau>" 
+    "\<exists>\<tau>. term.welltyped t \<tau> \<and> term.welltyped t'' \<tau>"
+    unfolding atomize_conj literal.typing_defs atom.typing_defs
+    by simp
 
-  hence t_t'_same_type: "\<exists>\<tau>. welltyped \<F> t' \<tau> \<and> welltyped \<F> t'' \<tau>"
-    using welltyped_right_unique[THEN right_uniqueD] by metis
+  hence t_t'_same_type: "\<exists>\<tau>. term.welltyped t' \<tau> \<and> term.welltyped t'' \<tau>"
+    using term.welltyped_right_unique[THEN right_uniqueD] 
+    by metis
 
   show ?thesis
-    unfolding \<open>C = add_mset (t' !\<approx> t'') (add_mset (t \<approx> t'') D')\<close> welltyped\<^sub>c_add_mset
+    unfolding \<open>C = add_mset (t' !\<approx> t'') (add_mset (t \<approx> t'') D')\<close> clause.is_welltyped_add_mset
   proof (intro conjI)
-    show "welltyped\<^sub>l \<F> (t' !\<approx> t'')"
+    show "literal.is_welltyped (t' !\<approx> t'')"
       using t_t'_same_type
-      unfolding welltyped\<^sub>l_def welltyped\<^sub>a_def by simp
+      unfolding literal.typing_defs atom.typing_defs 
+      by simp
   next
-    show "welltyped\<^sub>l \<F> (t \<approx> t'')"
-      using \<open>welltyped\<^sub>l \<F> (t \<approx> t'')\<close> .
+    show "literal.is_welltyped (t \<approx> t'')"
+      using \<open>literal.is_welltyped (t \<approx> t'')\<close> .
   next
-    show "welltyped\<^sub>c \<F> D'"
-      using \<open>welltyped\<^sub>c \<F> D'\<close> .
+    show "clause.is_welltyped D'"
+      using \<open>clause.is_welltyped D'\<close> .
   qed
 qed
+
+end
 
 end
