Superposition_Calculus/Ground_Typing.thy
@@ -1,0 +1,121 @@
+theory Ground_Typing
+  imports Ground_Clause Clause_Typing Term_Typing
+begin
+
+inductive typed for \<F> where
+  GFun: "\<F> f = (\<tau>s, \<tau>) \<Longrightarrow> typed \<F> (GFun f ts) \<tau>"
+
+inductive welltyped for \<F> where
+  GFun: "\<F> f = (\<tau>s, \<tau>) \<Longrightarrow> list_all2 (welltyped \<F>) ts \<tau>s \<Longrightarrow> welltyped \<F> (GFun f ts) \<tau>"
+
+locale ground_term_typing =
+  fixes \<F> :: "('f, 'ty) fun_types"
+begin
+
+sublocale typed_def where typed_def = "typed \<F>" and welltyped_def = "welltyped \<F>" .
+
+sublocale explicit_typing where typed = typed  and welltyped = welltyped
+proof unfold_locales
+  show "right_unique typed"
+  proof (rule right_uniqueI)
+    fix t \<tau>\<^sub>1 \<tau>\<^sub>2
+    assume "typed t \<tau>\<^sub>1" and "typed t \<tau>\<^sub>2"
+    thus "\<tau>\<^sub>1 = \<tau>\<^sub>2"
+      by (auto elim!: typed.cases)
+  qed
+next
+  show welltyped_right_unique: "right_unique welltyped"
+  proof (rule right_uniqueI)
+    fix t \<tau>\<^sub>1 \<tau>\<^sub>2
+    assume "welltyped t \<tau>\<^sub>1" and "welltyped t \<tau>\<^sub>2"
+    thus "\<tau>\<^sub>1 = \<tau>\<^sub>2"
+      by (auto elim!: welltyped.cases)
+  qed
+next
+  fix t \<tau>
+  assume "welltyped t \<tau>"
+  then show "typed t \<tau>"
+    by (metis typed.intros welltyped.cases)
+qed
+
+sublocale context_compatible_typing where 
+  typed = typed  and welltyped = welltyped and Fun = GFun
+proof unfold_locales
+  fix t t' c \<tau> \<tau>'
+  assume 
+    t_type: "welltyped t \<tau>'" and 
+    t'_type: "welltyped t' \<tau>'" and
+    c_type: "welltyped c\<langle>t\<rangle>\<^sub>G \<tau>"
+
+  from c_type show "welltyped c\<langle>t'\<rangle>\<^sub>G \<tau>"
+  proof (induction c arbitrary: \<tau>)
+    case Hole
+    then show ?case
+      using t_type t'_type welltyped_right_unique[THEN right_uniqueD]
+      by auto
+  next
+    case (More f ss1 c ss2)
+
+    have "welltyped (GFun f (ss1 @ c\<langle>t\<rangle>\<^sub>G # ss2)) \<tau>"
+      using More.prems 
+      by simp
+
+    hence "welltyped (GFun f (ss1 @ c\<langle>t'\<rangle>\<^sub>G # ss2)) \<tau>"
+    proof (cases \<F> "GFun f (ss1 @ c\<langle>t\<rangle>\<^sub>G # ss2)" \<tau> rule: welltyped.cases)
+      case (GFun \<tau>s)
+
+      show ?thesis
+      proof (rule welltyped.GFun)
+        show "\<F> f = (\<tau>s, \<tau>)"
+          using \<open>\<F> f = (\<tau>s, \<tau>)\<close> .
+      next
+        show "list_all2 welltyped (ss1 @ c\<langle>t'\<rangle>\<^sub>G # ss2) \<tau>s"
+          using \<open>list_all2 welltyped (ss1 @ c\<langle>t\<rangle>\<^sub>G # ss2) \<tau>s\<close>
+          using More.IH
+          by (smt (verit, del_insts) list_all2_Cons1 list_all2_append1 list_all2_lengthD)
+      qed
+    qed
+
+    thus ?case
+      by simp
+  qed
+next
+  fix t t' c \<tau> \<tau>'
+  assume 
+    t_type: "typed t \<tau>'" and 
+    t'_type: "typed t' \<tau>'" and
+    c_type: "typed c\<langle>t\<rangle>\<^sub>G \<tau>"
+ 
+  from c_type show "typed c\<langle>t'\<rangle>\<^sub>G \<tau>"
+  proof (induction c arbitrary: \<tau>)
+    case Hole
+    then show ?case
+      using t_type t'_type typed_right_unique[THEN right_uniqueD]
+      by auto
+  next
+    case (More f ss1 c ss2)
+
+    have "typed (GFun f (ss1 @ c\<langle>t\<rangle>\<^sub>G # ss2)) \<tau>"
+      using More.prems 
+      by simp
+
+    hence "typed (GFun f (ss1 @ c\<langle>t'\<rangle>\<^sub>G # ss2)) \<tau>"
+    proof (cases \<F> "GFun f (ss1 @ c\<langle>t\<rangle>\<^sub>G # ss2)" \<tau> rule: typed.cases)
+      case (GFun \<tau>s)
+
+      then show ?thesis
+        by (simp add: typed.simps)
+    qed
+
+    thus ?case
+      by simp
+  qed
+qed
+
+end
+
+locale ground_typing = 
+  "term": ground_term_typing + 
+  clause_typing where term_typed = term.typed and term_welltyped = term.welltyped
+
+end
