Superposition_Calculus/Term_Typing.thy
@@ -1,0 +1,27 @@
+theory Term_Typing
+  imports Typing Context_Extra
+begin
+
+type_synonym ('f, 'ty) fun_types = "'f \<Rightarrow> 'ty list \<times> 'ty"
+type_synonym ('v, 'ty) var_types = "'v \<Rightarrow> 'ty"
+
+locale context_compatible_typing = explicit_typing +
+  fixes Fun
+  assumes 
+    welltyped_context_compatible: 
+    "\<And>t t' c \<tau> \<tau>'.
+      welltyped t \<tau>' \<Longrightarrow>
+      welltyped t' \<tau>' \<Longrightarrow>
+      welltyped (Fun\<langle>c; t\<rangle>) \<tau> \<Longrightarrow>
+      welltyped (Fun\<langle>c; t'\<rangle>) \<tau>" and
+    typed_context_compatible: 
+    "\<And>t t' c \<tau> \<tau>'.
+      typed t \<tau>' \<Longrightarrow>
+      typed t' \<tau>' \<Longrightarrow>
+      typed (Fun\<langle>c; t\<rangle>) \<tau> \<Longrightarrow>
+      typed (Fun\<langle>c; t'\<rangle>) \<tau>"
+
+locale term_typing = 
+  explicit_typing + context_compatible_typing
+
+end
