Superposition_Calculus/Typing.thy
@@ -1,0 +1,130 @@
+theory Typing
+  imports Main
+begin
+
+locale typing =
+  fixes is_typed is_welltyped
+  assumes is_typed_if_is_welltyped: 
+    "\<And>expr. is_welltyped expr \<Longrightarrow> is_typed expr"
+
+locale explicit_typing =
+  fixes typed welltyped
+  assumes 
+    typed_right_unique: "right_unique typed" and
+    welltyped_right_unique: "right_unique welltyped" and
+    typed_if_welltyped: "\<And>expr \<tau>. welltyped expr \<tau> \<Longrightarrow> typed expr \<tau>"
+begin
+
+definition is_typed where
+  "is_typed expr \<equiv> \<exists>\<tau>. typed expr \<tau>"
+
+definition is_welltyped where
+  "is_welltyped expr \<equiv> \<exists>\<tau>. welltyped expr \<tau>"
+
+sublocale typing where is_typed = is_typed and is_welltyped = is_welltyped
+   using typed_if_welltyped
+   by unfold_locales (auto simp: is_typed_def is_welltyped_def)
+
+lemmas typing_defs = is_typed_def is_welltyped_def
+
+end
+
+locale uniform_explicit_typing_lifting = 
+  sub: explicit_typing where typed = typed_sub and welltyped = welltyped_sub
+for typed_sub welltyped_sub :: "'sub \<Rightarrow> 'ty \<Rightarrow> bool" +
+fixes 
+  to_set :: "'expr \<Rightarrow> 'sub set" 
+assumes
+  to_set_not_empty: "\<And>expr. to_set expr \<noteq> {}" (* TODO: Better here or in definitions? *)
+begin
+
+definition typed where
+  "typed expr \<tau> \<equiv> \<forall>sub \<in> to_set expr. typed_sub sub \<tau>"
+
+definition welltyped where
+  "welltyped expr \<tau> \<equiv> \<forall>sub \<in> to_set expr. welltyped_sub sub \<tau>"
+
+sublocale explicit_typing where typed = typed and welltyped = welltyped
+proof unfold_locales
+  show "right_unique typed"
+  proof(rule right_uniqueI)
+    fix expr \<tau> \<tau>'
+    assume "typed expr \<tau>" "typed expr \<tau>'"
+    
+    then show "\<tau> = \<tau>'"
+      using to_set_not_empty right_uniqueD[OF sub.typed_right_unique] 
+      unfolding typed_def
+      by blast
+  qed
+next
+   show "right_unique welltyped"
+  proof(rule right_uniqueI)
+    fix expr \<tau> \<tau>'
+    assume "welltyped expr \<tau>" "welltyped expr \<tau>'"
+    
+    then show "\<tau> = \<tau>'"
+      using to_set_not_empty right_uniqueD[OF sub.welltyped_right_unique] 
+      unfolding welltyped_def
+      by blast
+  qed
+next
+  fix expr \<tau>
+  assume "welltyped expr \<tau>"  
+  then show "typed expr \<tau>"
+    using sub.typed_if_welltyped
+    unfolding welltyped_def typed_def
+    by simp
+qed
+
+lemmas typing_defs = typed_def welltyped_def is_typed_def is_welltyped_def
+
+end
+
+locale typing_lifting =
+  sub: typing where is_typed = is_typed_sub and is_welltyped = is_welltyped_sub
+for is_typed_sub is_welltyped_sub :: "'sub \<Rightarrow> bool" +
+fixes 
+  to_set :: "'expr \<Rightarrow> 'sub set"
+begin
+
+definition is_typed where
+  "is_typed expr \<equiv> \<forall>sub \<in> to_set expr. is_typed_sub sub"
+
+definition is_welltyped where
+  "is_welltyped expr \<equiv> \<forall>sub \<in> to_set expr. is_welltyped_sub sub"
+
+sublocale typing where is_typed = is_typed and is_welltyped = is_welltyped
+proof unfold_locales
+  fix expr
+  assume "is_welltyped expr"
+  then show "is_typed expr"
+    unfolding is_typed_def is_welltyped_def
+    using sub.is_typed_if_is_welltyped
+    by blast
+qed
+
+lemmas typing_defs = is_typed_def is_welltyped_def
+
+end
+
+subsection\<open>Unified naming\<close> (* TODO ? *)
+
+locale typed_def =
+  fixes typed_def welltyped_def :: "'expr \<Rightarrow> 'ty \<Rightarrow> bool" 
+begin 
+
+abbreviation typed where "typed \<equiv> typed_def"
+abbreviation welltyped where "welltyped \<equiv> welltyped_def"
+
+end
+
+locale is_typed_def =
+  fixes is_typed_def is_welltyped_def :: "'expr \<Rightarrow> bool" 
+begin 
+
+abbreviation is_typed where "is_typed \<equiv> is_typed_def"
+abbreviation is_welltyped where "is_welltyped \<equiv> is_welltyped_def"
+
+end
+
+end
